fstar/treedem/MLS.TreeDEM.Message.Transcript.fst
@@ -8,7 +8,7 @@ open MLS.Crypto
 val compute_confirmed_transcript_hash:
   #bytes:Type0 -> {|crypto_bytes bytes|} ->
   wire_format_nt -> framed_content_nt bytes -> bytes -> bytes ->
-  result (lbytes bytes (hash_length #bytes))
+  result bytes
 let compute_confirmed_transcript_hash #bytes #cb wire_format msg signature interim_transcript_hash =
   let? signature = mk_mls_bytes signature "compute_confirmed_transcript_hash" "signature" in
   if not (msg.content.content_type = CT_commit) then
@@ -20,19 +20,17 @@ let compute_confirmed_transcript_hash #bytes #cb wire_format msg signature inter
       signature;
     }) in
     let hash_input = concat #bytes interim_transcript_hash serialized_msg in
-    if not (length hash_input < hash_max_input_length #bytes) then error ""
-    else return (hash_hash hash_input)
+    hash_hash hash_input
   )
 
 val compute_interim_transcript_hash:
   #bytes:Type0 -> {|crypto_bytes bytes|} ->
   bytes -> bytes ->
-  result (lbytes bytes (hash_length #bytes))
+  result bytes
 let compute_interim_transcript_hash #bytes #cb confirmation_tag confirmed_transcript_hash =
   let? confirmation_tag = mk_mls_bytes confirmation_tag "compute_interim_transcript_hash" "confirmation_tag" in
   let serialized_auth = serialize (interim_transcript_hash_input_nt bytes) ({
     confirmation_tag;
   }) in
   let hash_input = concat #bytes confirmed_transcript_hash serialized_auth in
-  if not (length hash_input < hash_max_input_length #bytes) then error ""
-  else return (hash_hash hash_input)
+  hash_hash hash_input
