fstar/treesync/proofs/MLS.TreeSync.Invariants.UnmergedLeaves.Proofs.fst
@@ -12,6 +12,7 @@ open MLS.TreeSync.ParentHash
 open MLS.TreeCommon
 open MLS.TreeCommon.Lemmas
 open MLS.MiscLemmas
+open MLS.Result
 
 #set-options "--fuel 1 --ifuel 1"
 
@@ -120,8 +121,8 @@ val leaf_at_tree_add:
   #l:nat -> #i:tree_index l ->
   t:treesync bytes tkt l i -> li:leaf_index l i -> content:leaf_node_nt bytes tkt -> li':leaf_index l i ->
   Lemma
-  (requires tree_add_pre t li)
-  (ensures leaf_at (tree_add t li content) li' == (if li = li' then Some content else leaf_at t li'))
+  (requires Success? (tree_add t li content))
+  (ensures leaf_at (Success?.v (tree_add t li content)) li' == (if li = li' then Some content else leaf_at t li'))
 let rec leaf_at_tree_add #bytes #bl #tkt #l #i t li content li' =
   match t with
   | TLeaf _ -> ()
@@ -149,8 +150,8 @@ val unmerged_leaf_consistent_tree_add_self:
   #l:nat -> #i:tree_index l ->
   t:treesync bytes tkt l i -> li:leaf_index l i{li < pow2 32} -> content:leaf_node_nt bytes tkt ->
   Lemma
-  (requires tree_add_pre t li)
-  (ensures unmerged_leaf_consistent (tree_add t li content) li)
+  (requires Success? (tree_add t li content))
+  (ensures unmerged_leaf_consistent (Success?.v (tree_add t li content)) li)
 let rec unmerged_leaf_consistent_tree_add_self #bytes #bl #tkt #l #i t li content =
   match t with
   | TLeaf _ -> ()
@@ -171,8 +172,8 @@ val unmerged_leaf_consistent_tree_add_other:
   #l:nat -> #i:tree_index l ->
   t:treesync bytes tkt l i -> li:leaf_index l i -> content:leaf_node_nt bytes tkt -> li':nat_lbytes 4 ->
   Lemma
-  (requires tree_add_pre t li /\ unmerged_leaf_consistent t li')
-  (ensures unmerged_leaf_consistent (tree_add t li content) li')
+  (requires Success? (tree_add t li content) /\ unmerged_leaf_consistent t li')
+  (ensures unmerged_leaf_consistent (Success?.v (tree_add t li content)) li')
 let rec unmerged_leaf_consistent_tree_add_other #bytes #bl #tkt #l #i t li content li' =
   match t with
   | TLeaf _ -> ()
@@ -191,8 +192,8 @@ val unmerged_leaves_ok_tree_add:
   #l:nat -> #i:tree_index l ->
   t:treesync bytes tkt l i -> li:leaf_index l i -> content:leaf_node_nt bytes tkt ->
   Lemma
-  (requires tree_add_pre t li /\ unmerged_leaves_ok t)
-  (ensures unmerged_leaves_ok (tree_add t li content))
+  (requires Success? (tree_add t li content) /\ unmerged_leaves_ok t)
+  (ensures unmerged_leaves_ok (Success?.v (tree_add t li content)))
 let rec unmerged_leaves_ok_tree_add #bytes #bl #tkt #l #i t li content =
   match t with
   | TLeaf _ -> ()
@@ -201,15 +202,16 @@ let rec unmerged_leaves_ok_tree_add #bytes #bl #tkt #l #i t li content =
     match opt_content with
     | None -> ()
     | Some cont -> (
+      let Success new_tree = tree_add t li content in
       unmerged_leaf_consistent_tree_add_self t li content;
       FStar.Classical.forall_intro (FStar.Classical.move_requires (unmerged_leaf_consistent_tree_add_other t li content));
       list_for_all_eq (unmerged_leaf_consistent t) cont.unmerged_leaves;
-      list_for_all_eq (unmerged_leaf_consistent (tree_add t li content)) (insert_sorted li cont.unmerged_leaves);
+      list_for_all_eq (unmerged_leaf_consistent new_tree) (insert_sorted li cont.unmerged_leaves);
       list_for_all_eq (unmerged_leaf_exists t) cont.unmerged_leaves;
-      list_for_all_eq (unmerged_leaf_exists (tree_add t li content)) (insert_sorted li cont.unmerged_leaves);
+      list_for_all_eq (unmerged_leaf_exists new_tree) (insert_sorted li cont.unmerged_leaves);
       FStar.Classical.forall_intro (mem_insert_sorted li cont.unmerged_leaves);
       unmerged_leaves_sorted_insert_sorted li cont.unmerged_leaves;
-      introduce forall x. List.Tot.mem x (insert_sorted li cont.unmerged_leaves) ==> Some? (leaf_at (tree_add t li content) x)
+      introduce forall x. List.Tot.mem x (insert_sorted li cont.unmerged_leaves) ==> Some? (leaf_at new_tree x)
       with (
         leaf_at_tree_add t li content x
       )
@@ -218,31 +220,39 @@ let rec unmerged_leaves_ok_tree_add #bytes #bl #tkt #l #i t li content =
 
 (*** Apply path ***)
 
+#push-options "--z3rlimit 100"
 val unmerged_leaves_ok_apply_path_aux:
   #bytes:Type0 -> {|crypto_bytes bytes|} -> #tkt:treekem_types bytes ->
   #l:nat -> #i:tree_index l -> #li:leaf_index l i ->
-  t:treesync bytes tkt l i -> p:pathsync bytes tkt l i li -> parent_parent_hash:mls_bytes bytes ->
+  t:treesync bytes tkt l i -> p:pathsync bytes tkt l i li -> parent_parent_hash:bytes ->
   Lemma
-  (requires apply_path_aux_pre #bytes t p (length #bytes parent_parent_hash) /\ unmerged_leaves_ok t)
-  (ensures unmerged_leaves_ok (apply_path_aux t p parent_parent_hash))
+  (requires
+    unmerged_leaves_ok t /\
+    Success? (apply_path_aux t p parent_parent_hash)
+  )
+  (ensures unmerged_leaves_ok (Success?.v (apply_path_aux t p parent_parent_hash)))
 let rec unmerged_leaves_ok_apply_path_aux #bytes #cb #tkt #l #i #li t p parent_parent_hash =
   match t, p with
   | TLeaf _, PLeaf ext_content -> ()
   | TNode _ left right, PNode opt_ext_content p_next ->
     let (child, sibling) = get_child_sibling t li in
-    let (new_opt_content, new_parent_parent_hash) = compute_new_np_and_ph opt_ext_content sibling parent_parent_hash in
+    let Success (new_opt_content, new_parent_parent_hash) = compute_new_np_and_ph opt_ext_content sibling parent_parent_hash in
     if is_left_leaf li then
       unmerged_leaves_ok_apply_path_aux left p_next new_parent_parent_hash
     else
       unmerged_leaves_ok_apply_path_aux right p_next new_parent_parent_hash
+#pop-options
 
 val unmerged_leaves_ok_apply_path:
   #bytes:Type0 -> {|crypto_bytes bytes|} -> #tkt:treekem_types bytes ->
   #l:nat -> #li:leaf_index l 0 ->
   t:treesync bytes tkt l 0 -> p:pathsync bytes tkt l 0 li ->
   Lemma
-  (requires apply_path_pre #bytes t p /\ unmerged_leaves_ok t)
-  (ensures unmerged_leaves_ok (apply_path t p))
+  (requires
+    Success? (apply_path t p) /\
+    unmerged_leaves_ok t
+  )
+  (ensures unmerged_leaves_ok (Success?.v (apply_path t p)))
 let unmerged_leaves_ok_apply_path #bytes #cb #tkt #l #li t p =
   unmerged_leaves_ok_apply_path_aux t p (root_parent_hash #bytes)
 
