fstar/treesync/proofs/MLS.TreeSync.Operations.Lemmas.fst
@@ -8,6 +8,7 @@ open MLS.TreeSync.NetworkTypes
 open MLS.TreeSync.Types
 open MLS.TreeSync.ParentHash
 open MLS.TreeSync.Operations
+open MLS.Result
 
 #set-options "--fuel 1 --ifuel 1"
 
@@ -16,8 +17,8 @@ val leaf_at_tree_add:
   #l:nat -> #i:tree_index l ->
   t:treesync bytes tkt l i -> li:leaf_index l i -> ln:leaf_node_nt bytes tkt -> li':leaf_index l i ->
   Lemma
-  (requires tree_add_pre t li)
-  (ensures leaf_at (tree_add t li ln) li' == (if li = li' then Some ln else leaf_at t li'))
+  (requires Success? (tree_add t li ln))
+  (ensures leaf_at (Success?.v (tree_add t li ln)) li' == (if li = li' then Some ln else leaf_at t li'))
 let rec leaf_at_tree_add #bytes #bl #tkt #l #i t li ln li' =
   match t with
   | TLeaf _ -> ()
@@ -31,16 +32,16 @@ let rec leaf_at_tree_add #bytes #bl #tkt #l #i t li ln li' =
 val leaf_at_apply_path_aux:
   #bytes:Type0 -> {|crypto_bytes bytes|} -> #tkt:treekem_types bytes ->
   #l:nat -> #i:tree_index l -> #li:leaf_index l i ->
-  t:treesync bytes tkt l i -> p:pathsync bytes tkt l i li -> parent_parent_hash:mls_bytes bytes -> li':leaf_index l i ->
+  t:treesync bytes tkt l i -> p:pathsync bytes tkt l i li -> parent_parent_hash:bytes -> li':leaf_index l i ->
   Lemma
-  (requires apply_path_aux_pre t p (length #bytes parent_parent_hash))
-  (ensures leaf_at (apply_path_aux t p parent_parent_hash) li' == (if li = li' then Some (get_path_leaf p) else leaf_at t li'))
+  (requires Success? (apply_path_aux t p parent_parent_hash))
+  (ensures leaf_at (Success?.v (apply_path_aux t p parent_parent_hash)) li' == (if li = li' then Some (get_path_leaf p) else leaf_at t li'))
 let rec leaf_at_apply_path_aux #bytes #cb #tkt #l #i #li t p parent_parent_hash li' =
   match t, p with
   | TLeaf _, PLeaf _-> ()
   | TNode _ left right, PNode opt_ext_content p_next -> (
     let (child, sibling) = get_child_sibling t li in
-    let (new_opt_content, new_parent_parent_hash) = compute_new_np_and_ph opt_ext_content sibling parent_parent_hash in
+    let Success (new_opt_content, new_parent_parent_hash) = compute_new_np_and_ph opt_ext_content sibling parent_parent_hash in
     match is_left_leaf li, is_left_leaf li' with
     | true, true -> leaf_at_apply_path_aux left p_next new_parent_parent_hash li'
     | false, false -> leaf_at_apply_path_aux right p_next new_parent_parent_hash li'
@@ -52,7 +53,7 @@ val leaf_at_apply_path:
   #l:nat -> #li:leaf_index l 0 ->
   t:treesync bytes tkt l 0 -> p:pathsync bytes tkt l 0 li -> li':leaf_index l 0 ->
   Lemma
-  (requires apply_path_pre t p)
-  (ensures leaf_at (apply_path t p) li' = (if li = li' then Some (get_path_leaf p) else leaf_at t li'))
+  (requires Success? (apply_path t p))
+  (ensures leaf_at (Success?.v (apply_path t p)) li' = (if li = li' then Some (get_path_leaf p) else leaf_at t li'))
 let leaf_at_apply_path #bytes #cb #tkt #l #li t p li' =
   leaf_at_apply_path_aux t p (root_parent_hash #bytes) li'
