fstar/treesync/symbolic/MLS.TreeSync.Symbolic.LeafNodeSignature.fst
@@ -20,6 +20,7 @@ open MLS.TreeSync.API.Types
 open MLS.TreeSync.Symbolic.IsWellFormed
 open MLS.TreeSync.Symbolic.Parsers
 open MLS.Symbolic
+open MLS.Result
 
 #set-options "--fuel 1 --ifuel 1"
 
@@ -468,25 +469,23 @@ let state_implies_event #tkt #group_id #l #i gu time st t ast =
 val external_path_to_path_aux_nosig:
   #bytes:Type0 -> {|crypto_bytes bytes|} -> #tkt:treekem_types bytes ->
   #l:nat -> #i:tree_index l -> #li:leaf_index l i ->
-  t:treesync bytes tkt l i -> p:external_pathsync bytes tkt l i li -> group_id:mls_bytes bytes ->
-  Pure (leaf_node_nt bytes tkt)
-  (requires external_path_to_path_pre t p group_id)
-  (ensures fun _ -> True)
+  t:treesync bytes tkt l i -> p:external_pathsync bytes tkt l i li{(get_path_leaf p).source == LNS_update} -> group_id:mls_bytes bytes ->
+  result (leaf_node_nt bytes tkt)
 let external_path_to_path_aux_nosig #bytes #cb #tkt #l #i #li t p group_id =
-  let computed_parent_hash = compute_leaf_parent_hash_from_path t p root_parent_hash in
+  let? computed_parent_hash = compute_leaf_parent_hash_from_path t p (root_parent_hash #bytes) in
+  let? computed_parent_hash = mk_mls_bytes computed_parent_hash "external_path_to_path_aux_nosig" "computed_parent_hash" in
   let lp = get_path_leaf p in
   let new_lp_data = { lp with source = LNS_commit; parent_hash = computed_parent_hash; } in
-  ({ data = new_lp_data; signature = empty #bytes } <: leaf_node_nt bytes tkt)
+  return ({ data = new_lp_data; signature = empty #bytes } <: leaf_node_nt bytes tkt)
 
 val external_path_to_path_nosig:
   #bytes:Type0 -> {|crypto_bytes bytes|} -> #tkt:treekem_types bytes ->
   #l:nat -> #i:tree_index l -> #li:leaf_index l i ->
-  t:treesync bytes tkt l i -> p:external_pathsync bytes tkt l i li -> group_id:mls_bytes bytes ->
-  Pure (pathsync bytes tkt l i li)
-  (requires external_path_to_path_pre t p group_id)
-  (ensures fun _ -> True)
+  t:treesync bytes tkt l i -> p:external_pathsync bytes tkt l i li{(get_path_leaf p).source == LNS_update} -> group_id:mls_bytes bytes ->
+  result (pathsync bytes tkt l i li)
 let external_path_to_path_nosig #bytes #cb #tkt #l #i #li t p group_id =
-  set_path_leaf p (external_path_to_path_aux_nosig t p group_id)
+  let? new_leaf_node = external_path_to_path_aux_nosig t p group_id in
+  return (set_path_leaf p new_leaf_node)
 
 val get_path_leaf_set_path_leaf:
   #bytes:Type0 -> {|bytes_like bytes|} -> #tkt:treekem_types bytes ->
@@ -502,11 +501,9 @@ let rec get_path_leaf_set_path_leaf #bytes #bl #tkt #l #i #li p ln =
 val compute_leaf_parent_hash_from_path_set_path_leaf:
   #bytes:Type0 -> {|crypto_bytes bytes|} -> #tkt:treekem_types bytes ->
   #l:nat -> #i:tree_index l -> #li:leaf_index l i ->
-  t:treesync bytes tkt l i -> p:external_pathsync bytes tkt l i li -> ln:leaf_node_nt bytes tkt -> parent_parent_hash:mls_bytes bytes ->
+  t:treesync bytes tkt l i -> p:external_pathsync bytes tkt l i li -> ln:leaf_node_nt bytes tkt -> parent_parent_hash:bytes ->
   Lemma
-  (requires compute_leaf_parent_hash_from_path_pre t p (length #bytes parent_parent_hash))
   (ensures
-    compute_leaf_parent_hash_from_path_pre t (set_path_leaf p ln) (length #bytes parent_parent_hash) /\
     compute_leaf_parent_hash_from_path t (set_path_leaf p ln) parent_parent_hash == compute_leaf_parent_hash_from_path t p parent_parent_hash
   )
 let rec compute_leaf_parent_hash_from_path_set_path_leaf #bytes #cb #tkt #l #i #li t p ln parent_parent_hash =
@@ -514,8 +511,10 @@ let rec compute_leaf_parent_hash_from_path_set_path_leaf #bytes #cb #tkt #l #i #
   | TLeaf _, PLeaf _ -> ()
   | TNode _ left right, PNode opt_ext_content p_next ->
     let (child, sibling) = get_child_sibling t li in
-    let (_,  new_parent_parent_hash) = compute_new_np_and_ph opt_ext_content sibling parent_parent_hash in
-    compute_leaf_parent_hash_from_path_set_path_leaf child p_next ln new_parent_parent_hash
+    match compute_new_np_and_ph opt_ext_content sibling parent_parent_hash with
+    | Success (_,  new_parent_parent_hash) ->
+      compute_leaf_parent_hash_from_path_set_path_leaf child p_next ln new_parent_parent_hash
+    | _ -> ()
 
 #push-options "--z3rlimit 25"
 val path_is_parent_hash_valid_external_path_to_path_nosig:
@@ -523,10 +522,13 @@ val path_is_parent_hash_valid_external_path_to_path_nosig:
   #l:nat -> #li:leaf_index l 0 ->
   t:treesync bytes tkt l 0 -> p:external_pathsync bytes tkt l 0 li -> group_id:mls_bytes bytes ->
   Lemma
-  (requires external_path_to_path_pre t p group_id)
-  (ensures path_is_parent_hash_valid t (external_path_to_path_nosig t p group_id))
+  (requires
+    (get_path_leaf p).source == LNS_update /\
+    Success? (external_path_to_path_nosig t p group_id)
+  )
+  (ensures path_is_parent_hash_valid t (Success?.v (external_path_to_path_nosig t p group_id)))
 let path_is_parent_hash_valid_external_path_to_path_nosig #bytes #cb #tkt #l #li t p group_id =
-  let new_lp = external_path_to_path_aux_nosig t p group_id in
+  let Success new_lp = external_path_to_path_aux_nosig t p group_id in
   get_path_leaf_set_path_leaf p new_lp;
   compute_leaf_parent_hash_from_path_set_path_leaf t p new_lp (root_parent_hash #bytes)
 #pop-options
@@ -563,10 +565,14 @@ val path_is_filter_valid_external_path_to_path_nosig:
   #l:nat -> #li:leaf_index l 0 ->
   t:treesync bytes tkt l 0 -> p:external_pathsync bytes tkt l 0 li -> group_id:mls_bytes bytes ->
   Lemma
-  (requires external_path_to_path_pre t p group_id /\ path_is_filter_valid t p)
-  (ensures path_is_filter_valid t (external_path_to_path_nosig t p group_id))
+  (requires
+    (get_path_leaf p).source == LNS_update /\
+    Success? (external_path_to_path_nosig t p group_id) /\
+    path_is_filter_valid t p
+  )
+  (ensures path_is_filter_valid t (Success?.v (external_path_to_path_nosig t p group_id)))
 let path_is_filter_valid_external_path_to_path_nosig #bytes #cb #tkt #l #li t p group_id =
-  let new_lp = external_path_to_path_aux_nosig t p group_id in
+  let Success new_lp = external_path_to_path_aux_nosig t p group_id in
   path_is_filter_valid_set_path_leaf t p new_lp
 #pop-options
 
@@ -581,19 +587,41 @@ let path_is_filter_valid_external_path_to_path #bytes #cb #tkt #l #li t p group_
 #pop-options
 *)
 
+val apply_path_aux_compute_leaf_parent_hash_from_path_both_succeed:
+  #bytes:Type0 -> {|crypto_bytes bytes|} -> #tkt:treekem_types bytes ->
+  #l:nat -> #i:tree_index l -> #li:leaf_index l i ->
+  t:treesync bytes tkt l i -> p:pathsync bytes tkt l i li -> parent_parent_hash:bytes ->
+  Lemma
+  (Success? (apply_path_aux t p parent_parent_hash) <==> Success? (compute_leaf_parent_hash_from_path t p parent_parent_hash))
+let rec apply_path_aux_compute_leaf_parent_hash_from_path_both_succeed #bytes #cb #tkt #l #i #li t p parent_parent_hash =
+  match t, p with
+  | TLeaf old_lp, PLeaf new_lp -> ()
+  | TNode _ left right, PNode opt_ext_content p_next ->
+    let (child, sibling) = get_child_sibling t li in
+    match compute_new_np_and_ph opt_ext_content sibling parent_parent_hash with
+    | Success (_,  new_parent_parent_hash) ->
+      apply_path_aux_compute_leaf_parent_hash_from_path_both_succeed child p_next new_parent_parent_hash
+    | _ -> ()
+
 val external_path_has_event:
   #tkt:treekem_types dy_bytes ->
   #l:nat -> #li:leaf_index l 0 ->
   prin:principal -> time:timestamp ->
   t:treesync dy_bytes tkt l 0 -> p:external_pathsync dy_bytes tkt l 0 li -> group_id:mls_bytes dy_bytes ->
   Pure prop
-  (requires external_path_to_path_pre t p group_id)
+  (requires
+    (get_path_leaf p).source == LNS_update /\
+    li < pow2 32 /\
+    Success? (external_path_to_path_nosig t p group_id)
+  )
   (ensures fun _ -> True)
 let external_path_has_event #tkt #l #li prin time t p group_id =
   //This lemma is useful to know that auth_ln.data.source == LNS_commit
   path_is_parent_hash_valid_external_path_to_path_nosig t p group_id;
-  let auth_p = external_path_to_path_nosig t p group_id in
+  let Success auth_p = external_path_to_path_nosig t p group_id in
   let auth_ln = get_path_leaf auth_p in
+  compute_leaf_parent_hash_from_path_set_path_leaf t p auth_ln (root_parent_hash #dy_bytes);
+  apply_path_aux_compute_leaf_parent_hash_from_path_both_succeed t auth_p (root_parent_hash #dy_bytes);
   leaf_node_has_event prin time ({data = auth_ln.data; group_id; leaf_index = li;}) /\
   tree_list_has_event prin time group_id (path_to_tree_list t auth_p)
 
@@ -613,7 +641,8 @@ val is_msg_external_path_to_path:
   sk:sign_private_key dy_bytes -> nonce:sign_nonce dy_bytes ->
   Lemma
   (requires
-    external_path_to_path_pre t p group_id /\
+    (get_path_leaf p).source == LNS_update /\
+    Success? (external_path_to_path t p group_id sk nonce) /\
     path_is_filter_valid t p /\
     unmerged_leaves_ok t /\
     external_path_has_event prin time t p group_id /\
@@ -626,9 +655,9 @@ val is_msg_external_path_to_path:
     get_label gu nonce == readers [p_id prin] /\
     has_leaf_node_tbs_invariant tkt gu
   )
-  (ensures is_well_formed _ (is_msg gu label time) (external_path_to_path t p group_id sk nonce))
+  (ensures is_well_formed _ (is_msg gu label time) (Success?.v (external_path_to_path t p group_id sk nonce)))
 let is_msg_external_path_to_path #tkt #l #li gu prin label time t p group_id sk nonce =
-  let computed_parent_hash = compute_leaf_parent_hash_from_path t p root_parent_hash in
+  let Success computed_parent_hash = compute_leaf_parent_hash_from_path t p (root_parent_hash #dy_bytes) in
   let ln_data = get_path_leaf p in
   let new_ln_data = { ln_data with source = LNS_commit; parent_hash = computed_parent_hash; } in
   let new_ln_tbs: leaf_node_tbs_nt dy_bytes tkt = ({data = new_ln_data; group_id; leaf_index = li;}) in
@@ -637,10 +666,12 @@ let is_msg_external_path_to_path #tkt #l #li gu prin label time t p group_id sk 
   let new_ln = ({ data = new_ln_data; signature = new_signature; } <: leaf_node_nt dy_bytes tkt) in
   let new_unsigned_ln = ({ data = new_ln_data; signature = empty #dy_bytes; } <: leaf_node_nt dy_bytes tkt) in
   let unsigned_path = set_path_leaf p new_unsigned_ln in
+  compute_leaf_parent_hash_from_path_set_path_leaf t p new_unsigned_ln (root_parent_hash #dy_bytes);
+  apply_path_aux_compute_leaf_parent_hash_from_path_both_succeed t unsigned_path (root_parent_hash #dy_bytes);
   path_is_parent_hash_valid_external_path_to_path_nosig t p group_id;
   path_is_filter_valid_external_path_to_path_nosig t p group_id;
   get_path_leaf_set_path_leaf p new_unsigned_ln;
-  pre_compute_leaf_parent_hash_from_path (is_msg gu label time) t p root_parent_hash;
+  pre_compute_leaf_parent_hash_from_path (is_msg gu label time) t p (root_parent_hash #dy_bytes);
   is_well_formed_get_path_leaf (is_msg gu label time) p;
   serialize_wf_lemma (leaf_node_tbs_nt dy_bytes tkt) (is_msg gu label time) ({data = new_ln_data; group_id; leaf_index = li;});
   let tl = path_to_tree_list t unsigned_path in
